Wrote some code in Session. The SOURCES listed in the Makefile now all verify (but don't yet compile, because there are missing definitions).

src/Cipher.dfy
@@ -15,50 +15,113 @@ module Cipher {
     | AWS_CRYPTOSDK_RSA_OAEP_SHA1_MGF1
     | AWS_CRYPTOSDK_RSA_OAEP_SHA256_MGF1
 
-  class AlgorithmProperties {
-      // The name of the digest algorithm used for the KDF, or None if no KDF is used.
-      const md_name: Option<string>
-      // The name of the symmetric cipher in use.
-      const cipher_name: string
-      // The name of the overall algorithm suite in use (for debugging purposes)
-      const alg_name: string
+  trait AlgorithmProperties {
+    // The name of the digest algorithm used for the KDF, or None if no KDF is used.
+    const md_name: Option<string>
+    // The name of the symmetric cipher in use.
+    const cipher_name: string
+    // The name of the overall algorithm suite in use (for debugging purposes)
+    const alg_name: string
 
-      // The length of the data key (that is, the key returned by the keyrings/CMMs)
-      const data_key_len: nat
-      /**
-      * The length of the key used to actually encrypt/decrypt data. This may differ
-      * if a KDF is in use.
-      */
-      const content_key_len: nat
-      // The IV length for this algorithm suite
-      const iv_len: nat
-      /**
-      * The AEAD tag length for this algorithm suite. Note that, currently, we only
-      * support stream-like ciphers that do not require padding, so the ciphertext
-      * size is equal to the plaintext size plus tag (and IV, if you pre/append IV).
-      */
-      const tag_len: nat
-      /**
-      * The length of the trailing signature. Zero if there is no trailing signature
-      * for this algorithm suite.
-      */
-      const signature_len: nat
+    // The length of the data key (that is, the key returned by the keyrings/CMMs)
+    const data_key_len: nat
+    /**
+    * The length of the key used to actually encrypt/decrypt data. This may differ
+    * if a KDF is in use.
+    */
+    const content_key_len: nat
+    // The IV length for this algorithm suite
+    const iv_len: nat
+    /**
+    * The AEAD tag length for this algorithm suite. Note that, currently, we only
+    * support stream-like ciphers that do not require padding, so the ciphertext
+    * size is equal to the plaintext size plus tag (and IV, if you pre/append IV).
+    */
+    const tag_len: nat
+    /**
+    * The length of the trailing signature. Zero if there is no trailing signature
+    * for this algorithm suite.
+    */
+    const signature_len: nat
 
-      /**
-      * The algorithm ID for this algorithm suite
-      */
-      const alg_id: AlgorithmID
+    /**
+    * The algorithm ID for this algorithm suite
+    */
+    const alg_id: AlgorithmID
+  }
 
-      /**
-      * Looks up and returns the algorithm properties for a particular algorithm ID.
-      * Returns null if alg_id is unknown.
-      */
-      static method AlgProperties(alg_id: AlgorithmID) returns (p: AlgorithmProperties?)
-        ensures p != null ==> p.alg_id == alg_id
+  class AlgorithmProperties_AES_128_GCM_IV12_AUTH16_KDNONE_SIGNONE extends AlgorithmProperties {
+    constructor ()
+      ensures alg_id == AES_128_GCM_IV12_AUTH16_KDNONE_SIGNONE
+    {
+      this.md_name := Some("NULL");
+      this.cipher_name := "aes_128_gcm";
+      this.alg_name := "AES_256_GCM_IV12_AUTH16_KDNONE_SIGNONE";
+      this.data_key_len := 128 / 8;
+      this.content_key_len := 128 / 8;
+      this.iv_len := 12;
+      this.tag_len := 16;
+      this.signature_len := 0;
+      this.alg_id := AES_128_GCM_IV12_AUTH16_KDNONE_SIGNONE;
+    }
+  }
+
+  class AlgorithmProperties_AES_256_GCM_IV12_AUTH16_KDNONE_SIGNONE extends AlgorithmProperties {
+    constructor ()
+      ensures alg_id == AES_256_GCM_IV12_AUTH16_KDNONE_SIGNONE
+    {
+      this.md_name := Some("NULL");
+      this.cipher_name := "aes_256_gcm";
+      this.alg_name := "AES_256_GCM_IV12_AUTH16_KDNONE_SIGNONE";
+      this.data_key_len := 256 / 8;
+      this.content_key_len := 256 / 8;
+      this.iv_len := 12;
+      this.tag_len := 16;
+      this.signature_len := 0;
+      this.alg_id := AES_256_GCM_IV12_AUTH16_KDNONE_SIGNONE;
+    }
+  }
+
+  /**
+  * Looks up and returns the algorithm properties for a particular algorithm ID.
+  * Returns null if alg_id is unknown.
+  */
+  method AlgProperties(id: AlgorithmID) returns (p: AlgorithmProperties?)
+    ensures p != null ==> p.alg_id == id
+  {
+    if id == AES_128_GCM_IV12_AUTH16_KDNONE_SIGNONE {
+      p := new AlgorithmProperties_AES_128_GCM_IV12_AUTH16_KDNONE_SIGNONE();
+    } else if id == AES_256_GCM_IV12_AUTH16_KDNONE_SIGNONE {
+      p := new AlgorithmProperties_AES_256_GCM_IV12_AUTH16_KDNONE_SIGNONE();
+    } else {
+      p := null;  // unknown
+    }
   }
 
   /**
   * Represents an ongoing sign or verify operation
   */
   class SignCtx { }
+
+  method GenRandom(buf: array<byte>) returns (r: Outcome)
+    modifies buf
+  {
+    var rc := RAND_bytes(buf, buf.Length);
+    if rc != 1 {
+      forall i | 0 <= i < buf.Length {
+        buf[i] := 0;
+      }
+      return AWS_CRYPTOSDK_ERR_CRYPTO_UNKNOWN;
+    }
+    return AWS_OP_SUCCESS;
+  }
+  // TODO: the following method belongs in some library somewhere
+  // A return code of 1 means success (how could this operation fail?)
+  method RAND_bytes(buf: array<byte>, n: nat) returns (rc: int)
+    requires n <= buf.Length
+    modifies buf
+
+  class content_key { }  // TODO
+
+  method DeriveKey(properties: AlgorithmProperties, dataKey: array<byte>, messageId: array<byte>) returns (r: Outcome, contentKey: content_key)
 }
