src/EncryptDecryptString.dfy
@@ -1,8 +1,9 @@
 include "StandardLibrary.dfy"
 include "AwsCrypto.dfy"
+include "Session.dfy"
 
 import opened StandardLibrary_ = StandardLibrary
-type Math = Aws.Math
+import Math = Aws.Math
 
 method Main()
 {
@@ -19,13 +20,13 @@ method EncryptThenDecrypt(arn: string, plaintext_original: string)
 
   var ciphertext := new byte[1024];
   var r, ciphertext_len := encrypt_string(arn, ciphertext, plaintext, plaintext.Length);
-  if r != Aws.SUCCESS { return; }
+  if r != Aws.AWS_OP_SUCCESS { return; }
   print ">> Encrypted to ciphertext of length ", ciphertext_len, "\n";
 
   var plaintext_result := new byte[1024];
   var plaintext_result_len;
   r, plaintext_result_len := decrypt_string(arn, plaintext_result, ciphertext, ciphertext_len);
-  if r != Aws.SUCCESS { return; }
+  if r != Aws.AWS_OP_SUCCESS { return; }
   print ">> Decrypted to plaintext of length ", plaintext_result_len, "\n";
 
   calc {
@@ -51,25 +52,25 @@ method encrypt_string(key_arn: string,
   requires ciphertext != plaintext
   requires plaintext_len <= plaintext.Length
   modifies ciphertext
-  ensures r == Aws.SUCCESS ==> ciphertext_len <= ciphertext.Length
-  ensures r == Aws.SUCCESS ==> ciphertext[..ciphertext_len] == Math.Encrypt(plaintext[..plaintext_len])
+  ensures r == Aws.AWS_OP_SUCCESS ==> ciphertext_len <= ciphertext.Length
+  ensures r == Aws.AWS_OP_SUCCESS ==> ciphertext[..ciphertext_len] == Math.Encrypt(plaintext[..plaintext_len])
 {
   var kms_keyring := new Aws.KmsKeyring.Build(key_arn);
 
   var cmm := new Aws.CryptoMaterialsManager(kms_keyring);
   kms_keyring.Release();
 
-  var session := new Aws.Session.FromCMM(Aws.EncryptMode, cmm);
+  var session := new Session.FromCMM(Aws.EncryptMode, cmm);
   cmm.Release();
 
   r := session.SetMessageSize(plaintext_len);
-  if r != Aws.SUCCESS { return; }
+  if r != Aws.AWS_OP_SUCCESS { return; }
 
   var plaintext_consumed;
   r, ciphertext_len, plaintext_consumed := session.Process(
     ciphertext, ciphertext.Length,
     plaintext, plaintext_len);
-  if r == Aws.SUCCESS {
+  if r == Aws.AWS_OP_SUCCESS {
     assert session.IsDone();
     assert plaintext_consumed == plaintext_len;
   }
@@ -83,8 +84,8 @@ method decrypt_string(key_arn: string,
   requires plaintext != ciphertext
   requires ciphertext_len <= ciphertext.Length
   modifies plaintext
-  ensures r == Aws.SUCCESS ==> plaintext_len <= plaintext.Length
-  ensures r == Aws.SUCCESS ==> plaintext[..plaintext_len] == Math.Decrypt(ciphertext[..ciphertext_len])
+  ensures r == Aws.AWS_OP_SUCCESS ==> plaintext_len <= plaintext.Length
+  ensures r == Aws.AWS_OP_SUCCESS ==> plaintext[..plaintext_len] == Math.Decrypt(ciphertext[..ciphertext_len])
 {
   var kms_keyring := new Aws.KmsKeyring.Build(key_arn);
 
@@ -100,7 +101,7 @@ method decrypt_string(key_arn: string,
     plaintext.Length,
     ciphertext,
     ciphertext_len);
-  if r == Aws.SUCCESS {
+  if r == Aws.AWS_OP_SUCCESS {
     assert session.IsDone();
     assert ciphertext_consumed == ciphertext_len;
   }
